cogent/isa/Test.thy
@@ -1,0 +1,40 @@
+theory Test
+  imports "AutoCorres.AutoCorres"
+begin
+
+
+lemma mask_31: "(0x7FFFFFFF :: 32 word) = mask 31"
+  by (simp add: mask_def)
+
+lemma not_mask_31: "(0x80000000 :: 32 word) = ~~ (mask 31)"
+  by (simp add: mask_def)
+
+lemma mask_1: "(0x00000001 :: 32 word) = mask 1"
+  by (simp add: mask_def)
+
+lemma not_mask_1: "(0xFFFFFFFE :: 32 word) = ~~ (mask 1)"
+  by (simp add: mask_def)
+
+lemma lshift1_mask31_eq_not_mask1: "(mask 31 :: 32 word) << Suc 0 = ~~ (mask 1)"
+  by (simp add: mask_def)
+
+lemma
+  fixes v :: "32 word"
+  shows
+  "(b0 && 1 || (v && 0x7FFFFFFF << Suc 0) >> Suc 0) && 0x7FFFFFFF ||
+   ((b1 && 0xFFFFFFFE || (v >> 31) && 1) && 1 << 31) =
+    v"
+  apply (simp add:
+      shiftl_over_and_dist shiftr_over_or_dist
+      mask_31 not_mask_31
+      mask_1 not_mask_1
+      lshift1_mask31_eq_not_mask1
+      mask_shift and_mask2
+      word_bits_conv word_bits_size
+      word_bool_alg.conj_disj_distrib2
+      word_bool_alg.disj.assoc
+      word_bool_alg.conj.assoc)
+  apply (simp add: shiftr_over_and_dist mask_shiftl_decompose and_not_mask[symmetric] mask_or_not_mask)
+  done
+
+end
